src/Decidable.v
@@ -3,6 +3,7 @@
 
 Require Import Coq.Arith.PeanoNat.
 Require Import Coq.Arith.Compare_dec.
+Require Import Coq.ZArith.BinInt.
 
 Class Decidable (P : Prop) := dec : {P} + {~P}.
 Arguments dec _%type_scope {_}.
@@ -11,6 +12,7 @@ Notation DecidableRel R := (forall x y, Decidable (R x y)).
 Notation DecidableEq T := (forall (x y: T), Decidable (x = y)).
 
 Global Instance dec_eq_nat : DecidableEq nat := Nat.eq_dec.
+Global Instance dec_eq_Z : DecidableEq Z := Z.eq_dec.
 Global Instance dec_le_nat : DecidableRel le := Compare_dec.le_dec.
 Global Instance dec_lt_nat : DecidableRel lt := Compare_dec.lt_dec.
 Global Instance dec_ge_nat : DecidableRel ge := Compare_dec.ge_dec.
